@prefix : <#> . 
@prefix rdf: <http://www.w3.org/1999/02/22-rdf-syntax-ns#> .
@prefix rdfs: <http://www.w3.org/2000/01/rdf-schema#> .
@prefix owl: <http://www.w3.org/2002/07/owl#> .
@prefix xsd: <http://www.w3.org/2001/XMLSchema#> .
@prefix dc: <http://purl.org/dc/elements/1.1/> .

@prefix zkp: <./zkp-o#> .
@prefix spok: <./zkp-o-spok#> .

<> a owl:Ontology ;
    dc:title "LegoGroth16" ;
    dc:date "2024-11-06" ;
    dc:creator []; # deleted for anon review
    dc:description """
This is an RDF vocabulary to model Dynamic Universal Accumulator's proof of set (non-) membership.
The Dynamic Universal Accumulator protocol is an instance of a proof protocol for proving that a (secret) value is member or non-member of a set of elements.
Following the particular protocol produces a corresponding proof.
That is, there is a class of proofs that were produced following the particular protocol.
                 """ .

###################
#    Instances    #
###################
:DynamicUniversalAccumulatorProtocol a :ZeroKnowledgeProofProtocol ; 
    rdfs:isDefinedBy <https://eprint.iacr.org/2020/777> ;
    rdfs:label "Dynamic Universal Accumulator (uAcc) protocol" ;
    rdfs:comment """
The Dynamic Universal Accumulator protocol:
A protocol to prove that a (secret) value is member or non-member of a set of elements.
                 """ .

####################
#      Classes     #
####################

:PoSNM a rdfs:Class;
    rdfs:subClassOf zkp:ZeroKnowledgeProofOfSetNonMembership;
    rdfs:isDefinedBy <https://eprint.iacr.org/2020/777> ;
    rdfs:label "Dynamic Universal Accumulator Proof of Set Non-Membership" ;
    rdfs:comment """
The class of zero-knowledge proofs of set non-membership produced from following the Dynamic Universal Accumulator protocol.
                 """ .
:ProvingKey a rdfs:Class ;
    rdfs:isDefinedBy <https://eprint.iacr.org/2019/142.pdf> ;
    rdfs:label "proving key of Dynamic Universal Accumulator PoSNM" .

:PublicKey a rdfs:Class ;
    rdfs:isDefinedBy <https://eprint.iacr.org/2019/142.pdf> ;
    rdfs:label "public key of Dynamic Universal Accumulator" .

:UniversalAccumulator a rdfs:Class ;
    rdfs:isDefinedBy <https://eprint.iacr.org/2019/142.pdf> ;
    rdfs:label "Dynamic Universal Accumulator" ;
    rdfs:comment """
The actual accumulator of a set of elements.
                 """ .

:UniversalAccumulatorParameters a rdfs:Class ;
    rdfs:isDefinedBy <https://eprint.iacr.org/2019/142.pdf> ;
    rdfs:label "Dynamic Universal Accumulator parameters" ;
    rdfs:comment """
The parameters of the accumulator.
                 """ .

:NonMembershipWitness a rdfs:Class ;
    rdfs:isDefinedBy <https://eprint.iacr.org/2019/142.pdf> ;
    rdfs:label "non-membership witness" ;
    rdfs:comment """
The non-membership witness used in the proof. It is derived from the secret element that is to be proven not to be a member of the set.
                 """ .

:RandomizedWitness a rdfs:Class ;
    rdfs:isDefinedBy <https://eprint.iacr.org/2019/142.pdf> ;
    rdfs:label "randomized witness" ;
    rdfs:comment """
The randomized witness used for proof verification.
                 """ .

:Commitments a rdfs:Class ;
    rdfs:isDefinedBy <https://eprint.iacr.org/2019/142.pdf> ;
    rdfs:label "commitments" ;
    rdfs:comment """
The commitments used in the proof.
                 """ .

:Responses a rdfs:Class ;
    rdfs:isDefinedBy <https://eprint.iacr.org/2019/142.pdf> ;
    rdfs:label "responses" ;
    rdfs:comment """
The responses from the proof, e.g., Schnorr Responses.
                 """ .


####################
#    Properties    #
####################

:hasProvingKey a rdf:Property ;
    rdfs:isDefinedBy <> ;
    rdfs:label "has proving key" ;
    rdfs:comment """
The property indicates that the (subject) Dynamic Universal Accumulator PoSNM has (object) proving key that should be used for verification of the proof. 
                 """ ;
    rdfs:domain :PoSNM ;
    rdfs:range  :ProvingKey .

:hasWitness a rdf:Property ;
    rdfs:isDefinedBy <> ;
    rdfs:label "has witness" ;
    rdfs:comment """
The property indicates that the (subject) Dynamic Universal Accumulator PoSNM has (object) witness, i.e. the (secret) value that the proof is about. 
                 """ ;
    rdfs:domain :PoSNM ;
    rdfs:range  zkp:Witness .

:hasAccumulator a rdf:Property ;
    rdfs:isDefinedBy <> ;
    rdfs:label "has accumulator" ;
    rdfs:comment """
The property indicates that the (subject) Dynamic Universal Accumulator PoSNM has (object) accumulator, i.e. the accumulated set of elements where non-membership is proven. 
                 """ ;
    rdfs:domain :PoSNM ;
    rdfs:range  :UniversalAccumulator .

:hasMaxSize a rdf:Property ;
    rdfs:isDefinedBy <> ;
    rdfs:label "has maximum size" ;
    rdfs:comment """
The property indicates that the (subject) Dynamic Universal Accumulator has (object) a maximum number of elements that it can accumulate.
                 """ ;
    rdfs:domain :UniversalAccumulator ;
    rdfs:range  xsd:nonNegativeInteger .

:hasParameters a rdf:Property ;
    rdfs:isDefinedBy <> ;
    rdfs:label "has parameters" ;
    rdfs:comment """
The property indicates that the (subject) Dynamic Universal Accumulator has (object) some parameters.
                 """ ;
    rdfs:domain :UniversalAccumulator ;
    rdfs:range  :UniversalAccumulatorParameters .

:P a rdf:Property ;
    rdfs:isDefinedBy <> ;
    rdfs:label "has parameters" ;
    rdfs:comment """
The property indicates that the (subject) Dynamic Universal Accumulator has parameter P with the (object) value.
                 """ ;
    rdfs:domain :UniversalAccumulatorParameters ;
    rdfs:range  xsd:base64Binary .

:P_tilde a rdf:Property ;
    rdfs:isDefinedBy <> ;
    rdfs:label "has parameters" ;
    rdfs:comment """
The property indicates that the (subject) Dynamic Universal Accumulator has (object) some parameters.
                 """ ;
    rdfs:domain :UniversalAccumulatorParameters ;
    rdfs:range  xsd:base64Binary .

:hasPublicKey a rdf:Property ;
    rdfs:isDefinedBy <> ;
    rdfs:label "has public key" ;
    rdfs:comment """
The property indicates that the (subject) Dynamic Universal Accumulator has (object) public key.
                 """ ;
    rdfs:domain :UniversalAccumulator ;
    rdfs:range  :PublicKey .

:hasValue a rdf:Property ; # ? maybe rdf:value would also work?
    rdfs:isDefinedBy <> ;
    rdfs:label "has value" ;
    rdfs:comment """
The property indicates that the (subject) Dynamic Universal Accumulator has (object) accumulated value.
That is, the value that results from accumulating all the member elements of the accumulator.
                 """ ;
    rdfs:domain :UniversalAccumulator ;
    rdfs:range  xsd:base64Binary .

:C a rdf:Property ; 
    rdfs:isDefinedBy <> ;
    rdfs:label "has parameter C" ;
    rdfs:comment """
The property indicates that the (subject) non-membership witness has a parameter C with (object) value.
                 """ ;
    rdfs:domain :NonMembershipWitness ;
    rdfs:range  xsd:base64Binary .

:d a rdf:Property ; 
    rdfs:isDefinedBy <> ;
    rdfs:label "has parameter d" ;
    rdfs:comment """
The property indicates that the (subject) non-membership witness has a parameter d with (object) value.
                 """ ;
    rdfs:domain :NonMembershipWitness ;
    rdfs:range  xsd:base64Binary .

:isWitnessOf a rdf:Property ; 
    rdfs:isDefinedBy <> ;
    rdfs:label "is witness of" ;
    rdfs:comment """
The property indicates that the (subject) non-membership witness is witness of the (object).
                 """ ;
    rdfs:domain :NonMembershipWitness ;
    rdfs:range  zkp:Witness .

:witnessesNotMemberOf a rdf:Property ; 
    rdfs:isDefinedBy <> ;
    rdfs:label "witnesses non-membership of" ;
    rdfs:comment """
The property indicates that the (subject) non-membership witness witnesses of secret value to not be a member of the (object) accumulator.
                 """ ;
    rdfs:domain :NonMembershipWitness ;
    rdfs:range  :UniversalAccumulator .

:hasRandomizedWitness a rdf:Property ; 
    rdfs:isDefinedBy <> ;
    rdfs:label "has randomized witness" ;
    rdfs:comment """
The property indicates that the (subject) Dynamic Universal Accumulator PoSNM has (object) randomized witness for proof verification. 
                 """ ;
    rdfs:domain :PoSNM ;
    rdfs:range  :RandomizedWitness .

:E_C a rdf:Property ; 
    rdfs:isDefinedBy <> ;
    rdfs:label "has randomized witness parameter C" ;
    rdfs:comment """
The property indicates that the (subject) randomized witness has randomized witness parameter C with (object) value. 
                 """ ;
    rdfs:domain :RandomizedWitness ;
    rdfs:range  xsd:base64Binary .

:E_d a rdf:Property ; 
    rdfs:isDefinedBy <> ;
    rdfs:label "has randomized witness parameter E_d" ;
    rdfs:comment """
The property indicates that the (subject) randomized witness has randomized witness parameter E_d with (object) value. 
                 """ ;
    rdfs:domain :RandomizedWitness ;
    rdfs:range  xsd:base64Binary .

:E_d_inv a rdf:Property ; 
    rdfs:isDefinedBy <> ;
    rdfs:label "has randomized witness parameter E_d_inv" ;
    rdfs:comment """
The property indicates that the (subject) randomized witness has randomized witness parameter E_d_inv with (object) value. 
                 """ ;
    rdfs:domain :RandomizedWitness ;
    rdfs:range  xsd:base64Binary .

:commitment_to_randomness_T_sigma a rdf:Property ; 
    rdfs:isDefinedBy <> ;
    rdfs:label "has commitment to randomness T_sigma" ;
    rdfs:comment """
The property indicates that the (subject) randomized witness has commitment to randomness T_sigma with (object) value. (cf. Schnorr commitment to randomness) 
                 """ ;
    rdfs:domain :RandomizedWitness ;
    rdfs:range  xsd:base64Binary .

:commitment_to_randomness_T_rho a rdf:Property ; 
    rdfs:isDefinedBy <> ;
    rdfs:label "has commitment to randomness T_rho" ;
    rdfs:comment """
The property indicates that the (subject) randomized witness has commitment to randomness T_rho with (object) value. (cf. Schnorr commitment to randomness)
                 """ ;
    rdfs:domain :RandomizedWitness ;
    rdfs:range  xsd:base64Binary .


:hasCommitments a rdf:Property ; 
    rdfs:isDefinedBy <> ;
    rdfs:label "has commitments" ;
    rdfs:comment """
The property indicates that the (subject) Dynamic Universal Accumulator PoSNM has (object) commitments. 
                 """ ;
    rdfs:domain :PoSNM ;
    rdfs:range  :Commitments . 

:R_E a rdf:Property ; 
    rdfs:isDefinedBy <> ;
    rdfs:label "includes R_E" ;
    rdfs:comment """
The property indicates that the (subject) commitments include (object) value of R_E.
                 """ ;
    rdfs:domain :Commitments ;
    rdfs:range  xsd:base64Binary .

:R_sigma a rdf:Property ; 
    rdfs:isDefinedBy <> ;
    rdfs:label "includes R_E" ;
    rdfs:comment """
The property indicates that the (subject) commitments include (object) value of R_E.
                 """ ;
    rdfs:domain :Commitments ;
    rdfs:range  xsd:base64Binary .

:R_rho a rdf:Property ; 
    rdfs:isDefinedBy <> ;
    rdfs:label "includes R_rho" ;
    rdfs:comment """
The property indicates that the (subject) commitments include (object) value of R_rho.
                 """ ;
    rdfs:domain :Commitments ;
    rdfs:range  xsd:base64Binary .
:R_delta_sigma a rdf:Property ; 
    rdfs:isDefinedBy <> ;
    rdfs:label "includes R_delta_sigma" ;
    rdfs:comment """
The property indicates that the (subject) commitments include (object) value of R_delta_sigma.
                 """ ;
    rdfs:domain :Commitments ;
    rdfs:range  xsd:base64Binary .
:R_delta_rho a rdf:Property ; 
    rdfs:isDefinedBy <> ;
    rdfs:label "includes R_delta_rho" ;
    rdfs:comment """
The property indicates that the (subject) commitments include (object) value of R_delta_rho.
                 """ ;
    rdfs:domain :Commitments ;
    rdfs:range  xsd:base64Binary .
:R_A a rdf:Property ; 
    rdfs:isDefinedBy <> ;
    rdfs:label "includes R_A" ;
    rdfs:comment """
The property indicates that the (subject) commitments include (object) value of R_A.
                 """ ;
    rdfs:domain :Commitments ;
    rdfs:range  xsd:base64Binary .
:R_B a rdf:Property ; 
    rdfs:isDefinedBy <> ;
    rdfs:label "includes R_B" ;
    rdfs:comment """
The property indicates that the (subject) commitments include (object) value of R_B.
                 """ ;
    rdfs:domain :Commitments ;
    rdfs:range  xsd:base64Binary .

:hasResponses a rdf:Property ; 
    rdfs:isDefinedBy <> ;
    rdfs:label "has responses" ;
    rdfs:comment """
The property indicates that the (subject) Dynamic Universal Accumulator PoSNM has (object) responses, e.g., Schnorr responses for secret values in the proof. 
                 """ ;
    rdfs:domain :PoSNM ;
    rdfs:range  :Responses . 

:s_sigma a rdf:Property ; 
    rdfs:isDefinedBy <> ;
    rdfs:label "includes response s_sigma" ;
    rdfs:comment """
The property indicates that the (subject) responses include (object) response value s_sigma.
                 """ ;
    rdfs:domain :Commitments ;
    rdfs:range  xsd:base64Binary .

:s_rho a rdf:Property ; 
    rdfs:isDefinedBy <> ;
    rdfs:label "includes response s_rho" ;
    rdfs:comment """
The property indicates that the (subject) responses include (object) response value s_rho.
                 """ ;
    rdfs:domain :Commitments ;
    rdfs:range  xsd:base64Binary .

:s_delta_sigma a rdf:Property ; 
    rdfs:isDefinedBy <> ;
    rdfs:label "includes response s_delta_sigma" ;
    rdfs:comment """
The property indicates that the (subject) responses include (object) response value s_delta_sigma.
                 """ ;
    rdfs:domain :Commitments ;
    rdfs:range  xsd:base64Binary .

:s_delta_rho a rdf:Property ; 
    rdfs:isDefinedBy <> ;
    rdfs:label "includes response s_delta_rho" ;
    rdfs:comment """
The property indicates that the (subject) responses include (object) response value s_delta_rho.
                 """ ;
    rdfs:domain :Commitments ;
    rdfs:range  xsd:base64Binary .

:s_u a rdf:Property ; 
    rdfs:isDefinedBy <> ;
    rdfs:label "includes response s_u" ;
    rdfs:comment """
The property indicates that the (subject) responses include (object) response value s_u.
                 """ ;
    rdfs:domain :Commitments ;
    rdfs:range  xsd:base64Binary .

:s_v a rdf:Property ; 
    rdfs:isDefinedBy <> ;
    rdfs:label "includes response s_v" ;
    rdfs:comment """
The property indicates that the (subject) responses include (object) response value s_v.
                 """ ;
    rdfs:domain :Commitments ;
    rdfs:range  xsd:base64Binary .

:s_w a rdf:Property ; 
    rdfs:isDefinedBy <> ;
    rdfs:label "includes response s_w" ;
    rdfs:comment """
The property indicates that the (subject) responses include (object) response value s_w.
                 """ ;
    rdfs:domain :Commitments ;
    rdfs:range  xsd:base64Binary .


