@prefix : <#> . 
@prefix rdf: <http://www.w3.org/1999/02/22-rdf-syntax-ns#> .
@prefix rdfs: <http://www.w3.org/2000/01/rdf-schema#> .
@prefix owl: <http://www.w3.org/2002/07/owl#> .
@prefix xsd: <http://www.w3.org/2001/XMLSchema#> .
@prefix dc: <http://purl.org/dc/elements/1.1/> .

@prefix cred: <https://www.w3.org/2018/credentials#> .

@prefix zkp: <./zkp-o#> .
@prefix spok: <./zkp-o-spok#> .


<> a owl:Ontology ;
    dc:title "BBS+ signature and proof of knowledge" ;
    dc:date "2024-11-06" ;
    dc:creator []; # deleted for anon review
    dc:description """
This is an RDF vocabulary to model BBS+ signatures and proof of knowledges.
The BBS+ scheme and proof protocol are instances of their respective generic classes.
Following the particular scheme and protocol produces corresponding signatures and proofs.
That is, there is a class of signatures and proofs that were produced following the particular scheme and protocol.
                 """ .

###################
#    Instances    #
###################
    
:SignatureScheme a zkp:MultiMessageSignatureScheme ; 
    rdfs:isDefinedBy <https://eprint.iacr.org/2016/663> ;
    rdfs:label "BBS+ signature scheme" ;
    rdfs:comment """
The "Boneh-Boyen-Shacham plus" signature scheme:
BBS signatures were implicitly proposed by Boneh, Boyen, and Shacham (CRYPTO '04) as part of their group signature scheme, and explicitly cast as stand-alone signatures by Camenisch and Lysyanskaya (CRYPTO '04). 
A provably secure version, called BBS+, was then devised by Au, Susilo, and Mu (SCN '06).
                 """ .

:PoksProtocol a zkp:NonInteractiveZeroKnowledgeProofProtocol ; 
    rdfs:isDefinedBy <https://eprint.iacr.org/2016/663> ;
    rdfs:label "protocol for proof of knowledge of BBS+ signature" ;
    rdfs:comment """
The "Boneh-Boyen-Shacham plus" proof of knowledge of signature protocol:
Protocol to construct a proof of knowledge of BBS plus signature from a BBS plus signature.
It can be used for selective disclosure of signed messages.
                 """ .

####################
#      Classes     #
####################

:Signature a rdfs:Class;
    rdfs:subClassOf zkp:MultiMessageSignature;
    rdfs:isDefinedBy <https://eprint.iacr.org/2016/663> ;
    rdfs:label "BBS+ signature" ;
    rdfs:comment """
The class of BBS+ signatures from following the BBS+ scheme.
                 """ .

:PoKS a rdfs:Class;
    rdfs:subClassOf zkp:ZeroKnowledgeProofOfKnowledgeOfSignature;
    rdfs:isDefinedBy <https://eprint.iacr.org/2016/663> ;
    rdfs:label "proof of Knowledge of BBS+ Signature" ;
    rdfs:comment """
The class of proofs of knowledge of BBS+ signature from following the BBS+ scheme.
                 """ .

:PublicKey a rdfs:Class ;
    rdfs:isDefinedBy <https://eprint.iacr.org/2016/663> ;
    rdfs:label "public key of (verification key and bases for) BBS+ Signature" ;
    rdfs:comment """
The paper defines the verification key to only be public parameter w, but we group all the public bases with that in the public key.
                 """ .

:SignatureParameters a rdfs:Class ;
    rdfs:isDefinedBy <> ;
    rdfs:label "parameters of a BBS+ Signature" ;
    rdfs:comment """
The class of parameters that may be used to create a BBS+ Signature.
                 """ .

:SPK1 a rdfs:Class;
    rdfs:subClassOf spok:SchnorrPok ;
    rdfs:isDefinedBy <https://eprint.iacr.org/2016/663> ;
    rdfs:label "Signature Proof of Knowledge (Part 1)" ;
    rdfs:comment """
The proof for the first part of the signature proof of knowledge from the paper. We use a SchnorrPoK.
                 """ .

:SPK2 a rdfs:Class;
    rdfs:subClassOf spok:SchnorrPok ;
    rdfs:isDefinedBy <https://eprint.iacr.org/2016/663> ;
    rdfs:label "Signature Proof of Knowledge (Part 2)" ;
    rdfs:comment """
The proof for the second part of the signature proof of knowledge from the paper. We use a SchnorrPoK.
                 """ .

####################
#    Properties    #
####################

:A_prime a rdf:Property ;
    rdfs:isDefinedBy <https://eprint.iacr.org/2016/663> ;
    rdfs:label "has parameter A prime" ;
    rdfs:comment """
The property indicates that the (subject) PoKS has an (object) A prime value.
                 """ ;
    rdfs:domain :PoKS ;
    rdfs:range  xsd:base64Binary .

:A_bar a rdf:Property ;
    rdfs:isDefinedBy <https://eprint.iacr.org/2016/663> ;
    rdfs:label "has parameter A bar" ;
    rdfs:comment """
The property indicates that the (subject) PoKS has an (object) A bar value.
                 """ ;
    rdfs:domain :PoKS ;
    rdfs:range  xsd:base64Binary .

:d  a rdf:Property ;
    rdfs:isDefinedBy <https://eprint.iacr.org/2016/663> ;
    rdfs:label "has parameter d" ;
    rdfs:comment """
The property indicates that the (subject) PoKS has an (object) d value.
                 """ ;
    rdfs:domain :PoKS ;
    rdfs:range  xsd:base64Binary .

:hasResponseValueFor_e  a rdf:Property ;
    rdfs:isDefinedBy <https://eprint.iacr.org/2016/663> ;
    rdfs:label "has response value for e" ;
    rdfs:comment """
The property indicates that the (subject) SPK1  has an (object) response value for signature parameter e.
                 """ ;
    rdfs:domain :SPK1 ;
    rdfs:range  xsd:base64Binary .

:hasResponseValueFor_r2 a rdf:Property ;
    rdfs:isDefinedBy <https://eprint.iacr.org/2016/663> ;
    rdfs:label "has response value for r2" ;
    rdfs:comment """
The property indicates that the (subject) SPK1  has an (object) response value for randomness r2.
                 """ ;
    rdfs:domain :SPK1 ;
    rdfs:range  xsd:base64Binary .

:hasResponseValueFor_r3 a rdf:Property ;
    rdfs:isDefinedBy <https://eprint.iacr.org/2016/663> ;
    rdfs:label "has response value for r3" ;
    rdfs:comment """
The property indicates that the (subject) SPK2  has an (object) response value for randomness r3.
                 """ ;
    rdfs:domain :SPK2 ;
    rdfs:range  xsd:base64Binary .

:hasResponseValueFor_a_prime  a rdf:Property ;
    rdfs:isDefinedBy <https://eprint.iacr.org/2016/663> ;
    rdfs:label "has response value for A prime" ;
    rdfs:comment """
The property indicates that the (subject) SPK2  has an (object) proof parameter value A prime.
                 """ ;
    rdfs:domain :SPK2 ;
    rdfs:range  xsd:base64Binary .

:hasSignatureParams  a rdf:Property ;
    rdfs:isDefinedBy <> ;
    rdfs:label "has response value for A prime" ;
    rdfs:comment """
The property indicates that the (subject) BBS+ public key is comprised of the (object) signature parameters.
                 """ ;
    rdfs:domain :PublicKey ;
    rdfs:range  :SignatureParameters .

:g1 a rdf:Property ;
    rdfs:isDefinedBy <https://eprint.iacr.org/2016/663> ;
    rdfs:label "has generator g1 of" ;
    rdfs:comment """
The property indicates that the (subject) signature parameters have the (object) g1 element, a generator of finite cyclic group G1.
                 """ ;
    rdfs:domain :SignatureParameters ;
    rdfs:range  xsd:base64Binary .

:g2 a rdf:Property ;
    rdfs:isDefinedBy <https://eprint.iacr.org/2016/663> ;
    rdfs:label "has generator g2 of" ;
    rdfs:comment """
The property indicates that the (subject) signature parameters have the (object) g2 element, a generator of finite cyclic group G2.
                 """ ;
    rdfs:domain :SignatureParameters ;
    rdfs:range  xsd:base64Binary .

:h_0 a rdf:Property ;
    rdfs:isDefinedBy <https://eprint.iacr.org/2016/663> ;
    rdfs:label "has base h_0 of" ;
    rdfs:comment """
The property indicates that the (subject) signature parameters have the (object) h_0 element, a randomly sampled element of finite cyclic group G1.
                 """ ;
    rdfs:domain :SignatureParameters ;
    rdfs:range  xsd:base64Binary .

:h_i a rdf:Property ;
    rdfs:isDefinedBy <https://eprint.iacr.org/2016/663> ;
    rdfs:label "has the list of h_i" ;
    rdfs:comment """
The property indicates that the (subject) signature parameters have a (object) list of h elements with index i, where all elements are randomly sampled from of finite cyclic group G1.
The length of the list, i.e. the value of i, is the (exact) number of messages that can be signed using the (subject) signature parameters. 
                 """ ;
    rdfs:domain :SignatureParameters ;
    rdfs:range  rdf:List .

:w a rdf:Property ;
    rdfs:isDefinedBy <https://eprint.iacr.org/2016/663> ;
    rdfs:label "has verification key w" ;
    rdfs:comment """
The property indicates that the (subject) signature parameters have the (object) w element, the verification key w = g2 ^ x with x being the secret key.
                 """ ;
    rdfs:domain :SignatureParameters ;
    rdfs:range  xsd:base64Binary .

:A a rdf:Property ;
    rdfs:isDefinedBy <https://eprint.iacr.org/2016/663> ;
    rdfs:label "has value for A of" ;
    rdfs:comment """
The property indicates that the (subject) signature proof value has the (object) value for A.
                 """ ;
    rdfs:domain cred:ProofValue ;
    rdfs:range  xsd:base64Binary .

:e a rdf:Property ;
    rdfs:isDefinedBy <https://eprint.iacr.org/2016/663> ;
    rdfs:label "has value for e of" ;
    rdfs:comment """
The property indicates that the (subject) signature proof value has the (object) value for e.
                 """ ;
    rdfs:domain cred:ProofValue ;
    rdfs:range  xsd:base64Binary .

:s a rdf:Property ;
    rdfs:isDefinedBy <https://eprint.iacr.org/2016/663> ;
    rdfs:label "has value for s of" ;
    rdfs:comment """
The property indicates that the (subject) signature proof value has the (object) value for s.
                 """ ;
    rdfs:domain cred:ProofValue ;
    rdfs:range  xsd:base64Binary .